pulse/share/steel/examples/pulse/lib/PulseHashTable.fst
@@ -34,7 +34,7 @@ type ht_t (s : pht_sig_us) = {
 let s_to_ps (s:pht_sig_us) : pht_sig
   = { keyt = s.keyt; valt = s.valt; hashf = (fun k -> US.v (s.hashf k)) }
 
-let models (s:pht_sig_us) (ps:pht_sig{ps==s_to_ps s}) (ht:ht_t s) (pht:pht ps) : vprop
+let models (s:pht_sig_us) (ht:ht_t s) (pht:pht_t (s_to_ps s)) : vprop
 = A.pts_to ht.contents full_perm pht.repr `star`
   pure (US.v ht.sz == pht.sz)
 
@@ -46,19 +46,19 @@ let modulo_us (v1 v2:US.t) (m:pos_us) (_:squash(US.fits (US.v v1 + US.v v2)))
   = (v1 + v2) % m
 
 ```pulse
-fn pulse_lookup_index (#s:pht_sig_us) (#ps:(p:pht_sig{p==s_to_ps s}))
-                      (#pht:(p:pht ps{not_full p.repr}))  
+fn pulse_lookup_index (#s:pht_sig_us)
+                      (#pht:(p:pht_t (s_to_ps s){not_full p.repr}))  
                       (ht:ht_t s) (k:s.keyt)
-  requires models s ps ht pht
+  requires models s ht pht
   returns  o:(o:option (s.valt & US.t){o == PHT.lookup_index_us pht k})
-  ensures  models s ps ht pht
+  ensures  models s ht pht
 {
   let cidx = canonical_index_us k ht.sz;
   let mut off = 0sz;
   let mut cont = true;
   let mut ret = None #(s.valt & US.t);
 
-  unfold (models s ps ht pht);
+  unfold (models s ht pht);
 
   while (let voff = !off; let vcont = !cont; (voff <= ht.sz && vcont = true)) 
   invariant b. exists (voff:US.t) (vcont:bool). (
@@ -69,7 +69,8 @@ fn pulse_lookup_index (#s:pht_sig_us) (#ps:(p:pht_sig{p==s_to_ps s}))
     pure (
       US.v ht.sz == pht.sz /\
       voff <= ht.sz /\
-      walk_get_idx #ps #pht.sz pht.repr (US.v cidx) k (US.v voff) == lookup_repr_index #ps #pht.sz pht.repr k /\
+      walk_get_idx #(s_to_ps s) #pht.sz pht.repr (US.v cidx) k (US.v voff) 
+        == lookup_repr_index #(s_to_ps s) #pht.sz pht.repr k /\
       b == (voff <= ht.sz && vcont = true)
     ))
   {
@@ -106,7 +107,7 @@ fn pulse_lookup_index (#s:pht_sig_us) (#ps:(p:pht_sig{p==s_to_ps s}))
       };
     };
   };
-  fold (models s ps ht pht);
+  fold (models s ht pht);
   assert (R.pts_to ret full_perm (PHT.lookup_index_us pht k));
   let o = !ret;
   o
@@ -114,14 +115,14 @@ fn pulse_lookup_index (#s:pht_sig_us) (#ps:(p:pht_sig{p==s_to_ps s}))
 ```
 
 ```pulse
-fn lookup (#s:pht_sig_us) (#ps:(p:pht_sig{p==s_to_ps s}))
-          (#pht:(p:pht ps{not_full p.repr}))  
+fn lookup (#s:pht_sig_us)
+          (#pht:(p:pht_t (s_to_ps s){not_full p.repr}))  
           (ht:ht_t s) (k:s.keyt)
-  requires models s ps ht pht
+  requires models s ht pht
   returns  o:(o:option s.valt{o == PHT.lookup pht k})
-  ensures  models s ps ht pht
+  ensures  models s ht pht
 {
-  let o = pulse_lookup_index #s #ps #pht ht k;
+  let o = pulse_lookup_index #s #pht ht k;
   match o {
     Some p -> { Some (fst p) }
     None -> { None #s.valt }
@@ -130,17 +131,17 @@ fn lookup (#s:pht_sig_us) (#ps:(p:pht_sig{p==s_to_ps s}))
 ```
 
 ```pulse
-fn insert (#s:pht_sig_us) (#ps:(p:pht_sig{p==s_to_ps s}))
-          (#pht:(p:pht ps{not_full p.repr})) 
+fn insert (#s:pht_sig_us)
+          (#pht:(p:pht_t (s_to_ps s){not_full p.repr})) 
           (ht:ht_t s) (k:s.keyt) (v:s.valt)
-  requires models s ps ht pht
-  ensures  models s ps ht (PHT.insert pht k v)
+  requires models s ht pht
+  ensures  models s ht (PHT.insert pht k v)
 {
   let cidx = canonical_index_us k ht.sz;
   let mut off = 0sz;
   let mut cont = true;
 
-  unfold (models s ps ht pht);
+  unfold (models s ht pht);
 
   while (let voff = !off; let vcont = !cont; (voff <= ht.sz && vcont = true)) 
   invariant b. exists (voff:US.t) (vcont:bool). (
@@ -152,8 +153,8 @@ fn insert (#s:pht_sig_us) (#ps:(p:pht_sig{p==s_to_ps s}))
       voff <= ht.sz /\
       strong_all_used_not_by pht.repr (US.v cidx) (US.v voff) k /\
       walk pht.repr (US.v cidx) k (US.v voff) == lookup_repr pht.repr k /\
-      insert_repr_walk #ps #pht.sz #pht.spec pht.repr k v (US.v voff) (US.v cidx) () () 
-        == insert_repr #ps #pht.sz #pht.spec pht.repr k v /\
+      insert_repr_walk #(s_to_ps s) #pht.sz #pht.spec pht.repr k v (US.v voff) (US.v cidx) () () 
+        == insert_repr #(s_to_ps s) #pht.sz #pht.spec pht.repr k v /\
       b == (voff <= ht.sz && vcont = true)
     ))
   {
@@ -170,7 +171,7 @@ fn insert (#s:pht_sig_us) (#ps:(p:pht_sig{p==s_to_ps s}))
           if (k' = k) {
             op_Array_Assignment ht.contents idx (mk_used_cell k v);
             cont := false;
-            assert (pure (insert_repr #ps #pht.sz #pht.spec pht.repr k v `Seq.equal` 
+            assert (pure (insert_repr #(s_to_ps s) #pht.sz #pht.spec pht.repr k v `Seq.equal` 
               Seq.upd pht.repr (US.v idx) (mk_used_cell k v))); 
           } else {
             off := voff + 1sz;
@@ -179,25 +180,25 @@ fn insert (#s:pht_sig_us) (#ps:(p:pht_sig{p==s_to_ps s}))
         Clean -> {
           op_Array_Assignment ht.contents idx (mk_used_cell k v);
           cont := false;
-          assert (pure (insert_repr #ps #pht.sz #pht.spec pht.repr k v `Seq.equal` 
+          assert (pure (insert_repr #(s_to_ps s) #pht.sz #pht.spec pht.repr k v `Seq.equal` 
             Seq.upd pht.repr (US.v idx) (mk_used_cell k v)));
         }
         Zombie -> {
-          fold (models s ps ht pht);
-          let o = pulse_lookup_index #s #ps #pht ht k;
-          unfold (models s ps ht pht);
+          fold (models s ht pht);
+          let o = pulse_lookup_index #s #pht ht k;
+          unfold (models s ht pht);
           match o {
             Some p -> {
               op_Array_Assignment ht.contents (snd p) Zombie;
               op_Array_Assignment ht.contents idx (mk_used_cell k v);
               cont := false;
-              assert (pure (insert_repr #ps #pht.sz #pht.spec pht.repr k v `Seq.equal` 
+              assert (pure (insert_repr #(s_to_ps s) #pht.sz #pht.spec pht.repr k v `Seq.equal` 
                 Seq.upd (Seq.upd pht.repr (US.v (snd p)) Zombie) (US.v idx) (mk_used_cell k v)));
             }
             None -> { 
               op_Array_Assignment ht.contents idx (mk_used_cell k v); 
               cont := false;
-              assert (pure (insert_repr #ps #pht.sz #pht.spec pht.repr k v 
+              assert (pure (insert_repr #(s_to_ps s) #pht.sz #pht.spec pht.repr k v 
                 `Seq.equal` Seq.upd pht.repr (US.v idx) (mk_used_cell k v)));
             }
           };
@@ -205,22 +206,22 @@ fn insert (#s:pht_sig_us) (#ps:(p:pht_sig{p==s_to_ps s}))
       };
     };
   };
-  fold (models s ps ht (PHT.insert pht k v));
+  fold (models s ht (PHT.insert pht k v));
 }
 ```
 
 ```pulse
-fn delete (#s:pht_sig_us) (#ps:(p:pht_sig{p==s_to_ps s}))
-          (#pht:pht ps) 
+fn delete (#s:pht_sig_us)
+          (#pht:pht_t (s_to_ps s)) 
           (ht:ht_t s) (k:s.keyt)
-  requires models s ps ht pht
-  ensures  models s ps ht (PHT.delete pht k)
+  requires models s ht pht
+  ensures  models s ht (PHT.delete pht k)
 {
   let cidx = canonical_index_us k ht.sz;
   let mut off = 0sz;
   let mut cont = true;
 
-  unfold (models s ps ht pht);
+  unfold (models s ht pht);
 
   while (let voff = !off; let vcont = !cont; (voff <= ht.sz && vcont = true))
   invariant b. exists (voff:US.t) (vcont:bool). (
@@ -232,8 +233,8 @@ fn delete (#s:pht_sig_us) (#ps:(p:pht_sig{p==s_to_ps s}))
       voff <= ht.sz /\
       all_used_not_by pht.repr (US.v cidx) (US.v voff) k /\
       walk pht.repr (US.v cidx) k (US.v voff) == lookup_repr pht.repr k /\
-      delete_repr_walk #ps #pht.sz #pht.spec pht.repr k (US.v voff) (US.v cidx) () () 
-        == delete_repr #ps #pht.sz #pht.spec pht.repr k /\
+      delete_repr_walk #(s_to_ps s) #pht.sz #pht.spec pht.repr k (US.v voff) (US.v cidx) () () 
+        == delete_repr #(s_to_ps s) #pht.sz #pht.spec pht.repr k /\
       b == (voff <= ht.sz && vcont = true)
     ))
   {
@@ -267,6 +268,6 @@ fn delete (#s:pht_sig_us) (#ps:(p:pht_sig{p==s_to_ps s}))
       };
     };
   };
-  fold (models s ps ht (PHT.delete pht k));
+  fold (models s ht (PHT.delete pht k));
 }
 ```
